Fix bugs in Double basis module and prove specs for to/fromString

basis/DoubleProgScript.sml
@@ -5,11 +5,11 @@
 open preamble
      ml_translatorLib ml_progLib basisFunctionsLib
      wordsTheory
-     Word8ArrayProgTheory;
+     CommandLineProgTheory;
 
 val _ = new_theory"DoubleProg";
 
-val _ = translation_extends "Word8ArrayProg";
+val _ = translation_extends "CommandLineProg";
 
 (* Double module -- translated *)
 
@@ -19,6 +19,85 @@ val () = generate_sigs := true;
 
 val _ = ml_prog_update (add_dec
   ``Dtabbrev unknown_loc [] "double" (Atapp [] (Short "word64"))`` I);
+
+val _ = ml_prog_update open_local_block;
+
+val concat_all_def = Define `
+  concat_all (a:word8) b c d e f g h =
+    concat_word_list [a;b;c;d;e;f;g;h]:64 word`
+
+val concat_all_impl = REWRITE_RULE [concat_word_list_def, dimindex_8, ZERO_SHIFT, WORD_OR_CLAUSES] concat_all_def;
+
+val _ = (next_ml_names := ["concat_all"]);
+val _ = translate concat_all_impl;
+
+val _ = ml_prog_update open_local_in_block;
+
+val _ = process_topdecs
+  `fun fromString s =
+    let
+      val iobuff = Word8Array.array 8 (Word8.fromInt 0);
+      val _ = #(double_fromString) s iobuff;
+      val a = Word8Array.sub iobuff 0;
+      val b = Word8Array.sub iobuff 1;
+      val c = Word8Array.sub iobuff 2;
+      val d = Word8Array.sub iobuff 3;
+      val e = Word8Array.sub iobuff 4;
+      val f = Word8Array.sub iobuff 5;
+      val g = Word8Array.sub iobuff 6;
+      val h = Word8Array.sub iobuff 7;
+    in
+      concat_all a b c d e f g h
+    end;` |> append_prog;
+
+val _ = ml_prog_update close_local_blocks;
+
+val _ = ml_prog_update open_local_block;
+
+val byte_0_def = Define `byte_0 (d:word64) = (w2w d):word8`;
+val byte_1_def = Define `byte_1 (d:word64) = (w2w (d >>> 8)):word8`;
+val byte_2_def = Define `byte_2 (d:word64) = (w2w (d >>> 16)):word8`;
+val byte_3_def = Define `byte_3 (d:word64) = (w2w (d >>> 24)):word8`;
+val byte_4_def = Define `byte_4 (d:word64) = (w2w (d >>> 32)):word8`;
+val byte_5_def = Define `byte_5 (d:word64) = (w2w (d >>> 40)):word8`;
+val byte_6_def = Define `byte_6 (d:word64) = (w2w (d >>> 48)):word8`;
+val byte_7_def = Define `byte_7 (d:word64) = (w2w (d >>> 56)):word8`;
+
+val _ = translate byte_0_def;
+val _ = translate byte_1_def;
+val _ = translate byte_2_def;
+val _ = translate byte_3_def;
+val _ = translate byte_4_def;
+val _ = translate byte_5_def;
+val _ = translate byte_6_def;
+val _ = translate byte_7_def;
+
+val is_0_byte_def = Define `
+  is_0_byte (c:word8) = (c = n2w 0)`;
+
+val _ = translate is_0_byte_def;
+
+val _ = ml_prog_update open_local_in_block;
+
+val _ = process_topdecs
+  `fun toString d =
+    let
+      val iobuff = Word8Array.array (256) (Word8.fromInt 0);
+      val _ = Word8Array.update iobuff 0 (byte_0 d);
+      val _ = Word8Array.update iobuff 1 (byte_1 d);
+      val _ = Word8Array.update iobuff 2 (byte_2 d);
+      val _ = Word8Array.update iobuff 3 (byte_3 d);
+      val _ = Word8Array.update iobuff 4 (byte_4 d);
+      val _ = Word8Array.update iobuff 5 (byte_5 d);
+      val _ = Word8Array.update iobuff 6 (byte_6 d);
+      val _ = Word8Array.update iobuff 7 (byte_7 d);
+      val _ = #(double_toString) "" iobuff;
+      val n = Option.valOf (Word8Array.find is_0_byte iobuff);
+    in
+        Word8Array.substring iobuff 0 n
+    end;` |> append_prog;
+
+val _ = ml_prog_update close_local_blocks;
 
 (* Ternary operations *)
 val _ = trans "fma" ``fp64_mul_add roundTiesToEven``;
@@ -38,130 +117,6 @@ val _ = trans "=" ``fp64_equal``;
 val _ = trans "abs" ``fp64_abs``;
 val _ = trans "sqrt" ``fp64_sqrt roundTiesToEven``;
 val _ = trans "~" ``fp64_negate``;
-
-(* Define exception for fromString function *)
-val _ = process_topdecs `
-  exception InvalidFloat;` |> append_prog
-
-val _ = ml_prog_update open_local_block;
-
-fun get_exn_conv name =
-  EVAL ``lookup_cons (Short ^name) ^(get_env (get_ml_prog_state ()))``
-  |> concl |> rand |> rand |> rand
-
-val InvalidFloat = get_exn_conv ``"InvalidFloat"``;
-
-val InvalidFloat_exn_def = Define `
-  InvalidFloat_exn v = (v = Conv (SOME ^InvalidFloat) [])`
-
-(* We allocate a "buffer" in which the FFI can store the double word;
-  8 times an 8 bit word *)
-val iobuff_e = ``(App Aw8alloc [Lit (IntLit 8); Lit (Word8 0w)])``
-val eval_thm = let
-  val env = get_ml_prog_state () |> ml_progLib.get_env
-  val st = get_ml_prog_state () |> ml_progLib.get_state
-  val new_st = ``^st with refs := ^st.refs ++ [W8array (REPLICATE 8 0w)]``
-  val goal = list_mk_icomb (prim_mk_const {Thy="ml_prog", Name="eval_rel"},
-    [st, env, iobuff_e, new_st, mk_var ("x", semanticPrimitivesSyntax.v_ty)])
-  val lemma = goal |> (EVAL THENC SIMP_CONV(srw_ss())[semanticPrimitivesTheory.state_component_equality])
-  val v_thm = prove(mk_imp(lemma |> concl |> rand, goal),
-    rpt strip_tac \\ rveq \\ match_mp_tac(#2(EQ_IMP_RULE lemma))
-    \\ asm_simp_tac bool_ss [])
-    |> GEN_ALL |> SIMP_RULE std_ss [] |> SPEC_ALL;
-  val v_tm = v_thm |> concl |> strip_comb |> #2 |> last
-  val v_def = define_abbrev false "iobuff_loc" v_tm
-in v_thm |> REWRITE_RULE [GSYM v_def] end
-
-val _ = ml_prog_update (add_Dlet eval_thm "iobuff" []);
-
-val concat_all_def = Define `
-  concat_all (a:word8) b c d e f g h =
-    concat_word_list [a;b;c;d;e;f;g;h]:64 word`
-
-val concat_all_impl = REWRITE_RULE [concat_word_list_def, dimindex_8] concat_all_def;
-
-val _ = (next_ml_names := ["concat_all"]);
-val _ = translate concat_all_impl;
-
-val _ = ml_prog_update open_local_in_block;
-
-val _ = process_topdecs
-  `fun fromString s =
-    let
-      val _ = #(double_fromString) s iobuff;
-      val a = Word8Array.sub iobuff 0;
-      val b = Word8Array.sub iobuff 1;
-      val c = Word8Array.sub iobuff 2;
-      val d = Word8Array.sub iobuff 3;
-      val e = Word8Array.sub iobuff 4;
-      val f = Word8Array.sub iobuff 5;
-      val g = Word8Array.sub iobuff 6;
-      val h = Word8Array.sub iobuff 7;
-    in
-      concat_all a b c d e f g h
-    end;` |> append_prog;
-
-val _ = ml_prog_update close_local_blocks;
-
-val _ = ml_prog_update open_local_block;
-
-(* We allocate a "buffer" in which the FFI can store the double word
-  as a string + some space to store the double word itself *)
-val iobuff_e = ``(App Aw8alloc [Lit (IntLit (8 + 255)); Lit (Word8 0w)])``
-val eval_thm = let
-  val env = get_ml_prog_state () |> ml_progLib.get_env
-  val st = get_ml_prog_state () |> ml_progLib.get_state
-  val new_st = ``^st with refs := ^st.refs ++ [W8array (REPLICATE (8+255) 0w)]``
-  val goal = list_mk_icomb (prim_mk_const {Thy="ml_prog", Name="eval_rel"},
-    [st, env, iobuff_e, new_st, mk_var ("x", semanticPrimitivesSyntax.v_ty)])
-  val lemma = goal |> (EVAL THENC SIMP_CONV(srw_ss())[semanticPrimitivesTheory.state_component_equality])
-  val v_thm = prove(mk_imp(lemma |> concl |> rand, goal),
-    rpt strip_tac \\ rveq \\ match_mp_tac(#2(EQ_IMP_RULE lemma))
-    \\ asm_simp_tac bool_ss [])
-    |> GEN_ALL |> SIMP_RULE std_ss [] |> SPEC_ALL;
-  val v_tm = v_thm |> concl |> strip_comb |> #2 |> last
-  val v_def = define_abbrev false "iobuff_loc" v_tm
-in v_thm |> REWRITE_RULE [GSYM v_def] end
-
-val _ = ml_prog_update (add_Dlet eval_thm "iobuff" []);
-
-val split_word8_def = Define `
-  split_word8 (w:word64) =
-    let
-      w1:word8 = w2w w;
-      w2:word8 = w2w (w << 8);
-      w3:word8 = w2w (w << 16);
-      w4:word8 = w2w (w << 24);
-      w5:word8 = w2w (w << 32);
-      w6:word8 = w2w (w << 40);
-      w7:word8 = w2w (w << 48);
-      w8:word8 = w2w (w << 56);
-    in
-      (w1,w2,w3,w4,w5,w6,w7,w8)`
-
-val _ = (next_ml_names := ["split_word8"]);
-val _ = translate split_word8_def;
-
-val _ = ml_prog_update open_local_in_block;
-
-val _ = process_topdecs
-  `fun toString d =
-    let
-      val (w1,w2,w3,w4,w5,w6,w7,w8) = split_word8 d;
-      val _ = Word8Array.update iobuff 0 w1;
-      val _ = Word8Array.update iobuff 1 w2;
-      val _ = Word8Array.update iobuff 2 w3;
-      val _ = Word8Array.update iobuff 3 w4;
-      val _ = Word8Array.update iobuff 4 w5;
-      val _ = Word8Array.update iobuff 5 w6;
-      val _ = Word8Array.update iobuff 6 w7;
-      val _ = Word8Array.update iobuff 7 w8;
-      val _ = #(double_toString) s iobuff;
-    in
-      Word8Array.substring iobuff 8 (255 + 7)
-    end;` |> append_prog;
-
-val _ = ml_prog_update close_local_blocks;
 
 val _ = ml_prog_update (close_module NONE);
 
