basis/DoubleProofScript.sml
@@ -1,0 +1,233 @@
+(*
+  Proofs that the Double basis module behaves correctly
+*)
+open preamble
+     ml_translatorTheory ml_translatorLib ml_progLib cfLib
+     Word8ArrayProgTheory
+     Word8ArrayProofTheory
+     OptionProgTheory
+     DoubleFFITheory
+     DoubleProgTheory;
+
+val _ = new_theory "DoubleProof";
+
+val _ = translation_extends "DoubleProg";
+
+val basis_st = get_ml_prog_state;
+
+val doubleFuns_ok_def = Define `
+  doubleFuns_ok doubleFns =
+    (! w.
+      LENGTH (doubleFns.toString w) <= 256 /\
+      ~ MEM (CHR 0) (doubleFns.toString w))`;
+
+val DoubleIO_def = Define `
+  DoubleIO doubleFns =
+    IOx double_ffi_part doubleFns * (cond (doubleFuns_ok doubleFns))`;
+
+Theorem one_one_eq[simp]:
+  one x ==>> one y <=> x = y
+Proof
+  fs[SEP_IMP_def, one_def]
+QED
+
+Theorem MAP_CHR_w2n_n2w_ORD_id:
+  MAP (CHR o (w2n:word8 -> num) o (n2w:num -> word8) o ORD) s = s
+Proof
+  rewrite_tac[miscTheory.CHR_w2n_n2w_ORD]
+  \\ Induct_on `s`  \\ fs[MAP]
+QED
+
+Theorem into_bytes_len:
+  ! w. LENGTH (into_bytes n w) = n
+Proof
+  Induct_on `n` \\ fs[into_bytes_def]
+QED
+
+Theorem concat_all_into_bytes_id:
+  concat_all (HD (into_bytes 8 w)) (EL 1 (into_bytes 8 w))
+    (EL 2 (into_bytes 8 w)) (EL 3 (into_bytes 8 w)) (EL 4 (into_bytes 8 w))
+    (EL 5 (into_bytes 8 w)) (EL 6 (into_bytes 8 w)) (EL 7 (into_bytes 8 w)) = w
+Proof
+  fs[EVAL ``into_bytes 8 w``]
+  \\ fs[concat_all_def]
+  \\ blastLib.BBLAST_TAC
+QED
+
+Theorem double_fromString_spec:
+  ! s sv.
+  STRING_TYPE (strlit s) sv ==>
+  app (p:'ffi ffi_proj) Double_fromString_v [sv]
+    (DoubleIO df)
+    (POSTv v. cond (WORD (df.fromString s) v) * DoubleIO df)
+Proof
+  xcf_with_def "Double.fromString" Double_fromString_v_def
+  \\ reverse (Cases_on `doubleFuns_ok df`)
+  >- (fs[DoubleIO_def] \\ xpull)
+  \\ ntac 2 (xlet_auto >- (fs[] \\ xsimpl))
+  \\ rename [`W8ARRAY iobuff`]
+  \\ xlet `POSTv v. W8ARRAY iobuff (into_bytes 8 (df.fromString s)) * DoubleIO df`
+  >- (fs[DoubleIO_def, IOx_def, double_ffi_part_def, IO_def, mk_ffi_next_def]
+      \\ xpull \\ xffi \\ xsimpl
+      \\ fs[STRING_TYPE_def] \\ rveq
+      \\ qexists_tac `MAP (n2w o ORD) s` \\ fs[MAP_MAP_o]
+      \\ qexists_tac `emp`
+      \\ xsimpl
+      \\ rewrite_tac [one_one_eq] \\ fs[]
+      \\ conj_tac
+      >- (fs[MAP_CHR_w2n_n2w_ORD_id])
+      \\ fs[mk_ffi_next_def, ffi_fromString_def]
+      \\ xsimpl
+      \\ rewrite_tac [one_one_eq] \\ fs[MAP_MAP_o, MAP_CHR_w2n_n2w_ORD_id])
+  \\ ntac 8
+    (xlet_auto
+    >- (xsimpl \\ TRY (qexists_tac `df`) \\ fs[into_bytes_len]))
+  \\ xapp
+  \\ xsimpl
+  \\ ntac 8 (asm_exists_tac\\ fs[])
+  \\ rpt strip_tac
+  \\ Cases_on `df` \\ fs[doubleFuns_ok_def, WORD_def, concat_all_into_bytes_id]
+QED
+
+Theorem concat_all_bytes_i:
+  concat_all (byte_0 w) (byte_1 w) (byte_2 w) (byte_3 w) (byte_4 w) (byte_5 w)
+(byte_6 w) (byte_7 w) = w
+Proof
+  fs[concat_all_def, byte_0_def, byte_1_def, byte_2_def,
+     byte_3_def, byte_4_def, byte_5_def, byte_6_def, byte_7_def,
+     concat_word_list_def]
+  \\ blastLib.BBLAST_TAC
+QED
+
+Theorem firsti_app:
+  ! f s1 s2 n.
+    firsti f s1 = NONE /\
+    firsti f s2 = SOME n ==>
+    firsti f (s1 ++ s2) = SOME (n + LENGTH s1)
+Proof
+  Induct_on `s1` \\ fs[firsti_def] \\ rpt strip_tac \\ fs[]
+  \\ Cases_on `f h` \\ fs[]
+  \\ Cases_on `firsti f s1` \\ fs[]
+  \\ res_tac \\ fs[]
+QED
+
+Theorem firsti_app2:
+  ! f s1 s2 n.
+    firsti f s1 = SOME n ==>
+    firsti f (s1 ++ s2) = SOME n
+Proof
+  Induct_on `s1` \\ fs[firsti_def] \\ rpt strip_tac
+  \\ Cases_on `f h` \\ fs[]
+  \\ Cases_on `firsti f s1` \\ fs[]
+  \\ res_tac \\ rveq \\ fs[]
+QED
+
+Theorem firsti_none:
+  ~ MEM #"\^@" s ==>
+  firsti is_0_byte (MAP (n2w o ORD) s) = NONE
+Proof
+  Induct_on `s` \\ fs[firsti_def, is_0_byte_def]
+  \\ rpt strip_tac
+  \\ `ORD h MOD 256 = ORD h`
+    by (irule MOD_UNIQUE
+        \\ qexists_tac `0` \\ fs[ORD_BOUND])
+  \\ pop_assum (fn thm => fs[thm])
+  \\ fs[ORD_eq_0]
+QED
+
+Theorem toString_has_0byte:
+  ! w. doubleFuns_ok df /\
+  s = df.toString w ==>
+  firsti is_0_byte (MAP (n2w ∘ ORD) s ++ [0w] ++ remStr) =
+    SOME (LENGTH s)
+Proof
+  rpt strip_tac
+  \\ Q.ISPECL_THEN [`is_0_byte`] assume_tac firsti_app2
+  \\ first_x_assum (qspecl_then [`MAP (n2w o ORD) s ++ [0w]`, `remStr`, `STRLEN s`] assume_tac)
+  \\ first_x_assum irule
+  \\ Q.ISPECL_THEN [`is_0_byte`] assume_tac firsti_app
+  \\ first_x_assum (qspecl_then [`MAP (n2w o ORD) s`, `[0w]`, `0`] assume_tac)
+  \\ fs[doubleFuns_ok_def] \\ first_x_assum (qspec_then `w` assume_tac)
+  \\ fs[]
+  \\ IMP_RES_TAC firsti_none
+  \\ rveq \\ res_tac \\ fs[firsti_def, is_0_byte_def]
+QED
+
+Theorem TAKE_STRLEN_id:
+  TAKE (STRLEN s1) (MAP f s1 ++ s2) = MAP f s1
+Proof
+  Induct_on `s1` \\ fs[TAKE]
+QED
+
+Theorem TAKE_STRLEN_id2:
+  TAKE (STRLEN s1) (MAP f s1 ++ s2 ++ s3) = MAP f s1
+Proof
+  Induct_on `s1` \\ fs[TAKE]
+QED
+
+Theorem double_toString_spec:
+  ! (w:word64) wv.
+  WORD w wv ==>
+  app (p:'ffi ffi_proj) Double_toString_v [wv]
+    (DoubleIO df)
+    (POSTv v. cond (STRING_TYPE (implode (df.toString w)) v) * DoubleIO df)
+Proof
+  xcf_with_def "Double.toString" Double_toString_v_def
+  \\ reverse (Cases_on `doubleFuns_ok df`)
+  >- (fs[DoubleIO_def] \\ xpull)
+  \\ ntac 18 (xlet_auto >- (fs[] \\ xsimpl))
+  \\ rename [`W8ARRAY iobuff`]
+  \\ fs[concat_all_bytes_i]
+  \\ qabbrev_tac `res_str = df.toString w`
+  \\ qabbrev_tac `updBuf = (LUPDATE (byte_7 w) 7
+             (LUPDATE (byte_6 w) 6
+                (LUPDATE (byte_5 w) 5
+                   (LUPDATE (byte_4 w) 4
+                      (LUPDATE (byte_3 w) 3
+                         (LUPDATE (byte_2 w) 2
+                            (LUPDATE (byte_1 w) 1
+                               (LUPDATE (byte_0 w) 0 (REPLICATE 256 0w)))))))))`
+  \\ qabbrev_tac `final_str = (MAP (n2w o ORD) (res_str ++ [CHR 0]) ++
+                    DROP (LENGTH res_str + 1) updBuf):word8 list`
+  \\ xlet `POSTv v. W8ARRAY iobuff final_str * DoubleIO df`
+  >- (fs[DoubleIO_def, IOx_def, double_ffi_part_def, IO_def, mk_ffi_next_def]
+      \\ xpull \\ xffi \\ xsimpl
+      \\ qexists_tac `emp`
+      \\ fs [SEP_CLAUSES, one_one_eq]
+      \\ fs [mk_ffi_next_def, ffi_toString_def]
+      \\ unabbrev_all_tac
+      \\ fs [EVAL ``REPLICATE 256 x``]
+      \\ fs [EL_LUPDATE, HD_LUPDATE]
+      \\ fs[concat_all_bytes_i]
+      \\ xsimpl \\ fs[one_one_eq])
+  \\ xlet `POSTv v. W8ARRAY iobuff final_str *
+          DoubleIO df *
+          cond (OPTION_TYPE NUM (firsti is_0_byte final_str) v)`
+    >- (xapp \\ xsimpl
+        \\ qexists_tac `is_0_byte` \\ fs[is_0_byte_v_thm])
+  \\ IMP_RES_TAC toString_has_0byte
+  \\ first_x_assum (qspecl_then [`w`, `df.toString w`] assume_tac)
+  \\ fs[]
+  \\ xlet_auto \\ fs[]
+  >- (xsimpl
+      \\ unabbrev_all_tac
+      \\ fs[concat_all_bytes_i])
+  \\ xapp
+  \\ xsimpl
+  \\ once_rewrite_tac [CONJ_COMM] \\ rewrite_tac [GSYM CONJ_ASSOC]
+  \\ asm_exists_tac \\ fs[]
+  \\ rpt conj_tac
+  >- (rpt strip_tac
+      \\ fs[STRING_TYPE_def, mlstringTheory.implode_def]
+      \\ `firsti is_0_byte final_str = SOME (STRLEN (df.toString w))`
+          by (unabbrev_all_tac \\ fs[])
+      \\ fs[]
+      \\ `TAKE (STRLEN (df.toString w)) final_str = MAP (n2w o ORD) (df.toString w)`
+        by (unabbrev_all_tac \\ fs[concat_all_bytes_i, TAKE_STRLEN_id2])
+      \\ unabbrev_all_tac \\ fs[]
+      \\ fs[MAP_MAP_o, MAP_CHR_w2n_n2w_ORD_id])
+  \\ unabbrev_all_tac
+  \\ fs[]
+QED
+
+val _ = export_theory ();
